src/HOL/SMT_Examples/SMT_Word_Translation_Examples.thy
@@ -11,9 +11,199 @@ declare[[smt_expert_debug_alethe_level=0]]
 declare[[smt_nat_as_int=true,smt_trace]]
 
 
-lemma "(27 :: 4 word) = -5"
-  
+(*
+Overflows should be normalized before generating the SMT-LIB problem.
+*)
+lemma "(1705 :: 8 word) = 169"
+  apply (test_smt_translate 
+\<open>
+(set-logic AUFBVLIRAFS)
+(assert (! (not (= (_ bv169 8) (_ bv169 8))) :named a0))
+\<close>)  
   by (smt (cvc5))
+
+
+(*
+- is translated into bvneg
+*)
+lemma "(- 169 :: 8 word) = 87"
+  apply (test_smt_translate 
+\<open>
+(set-logic AUFBVLIRAFS)
+(assert (! (not (= (bvneg (_ bv169 8)) (_ bv87 8))) :named a0))
+\<close>)
+  by (smt (cvc5))
+
+(*
+\<le> is translated into bvule
+*)
+lemma "(42 :: 8 word) \<le> 43"
+  apply (test_smt_translate 
+\<open>
+(set-logic AUFBVLIRAFS)
+(assert (! (not (bvule (_ bv42 8) (_ bv43 8))) :named a0))
+\<close>)
+  by (smt (cvc5))
+
+(*
+< is translated into bvult
+*)
+lemma "(42 :: 8 word) < 43"
+  apply (test_smt_translate 
+\<open>
+(set-logic AUFBVLIRAFS)
+(assert (! (not (bvult (_ bv42 8) (_ bv43 8))) :named a0))
+\<close>)
+  by (smt (cvc5))
+
+(*
+\<le>s is translated into bvsle
+*)
+lemma "(42 :: 8 word) \<le>s 44"
+  apply (test_smt_translate 
+\<open>
+(set-logic AUFBVLIRAFS)
+(assert (! (not (bvsle (_ bv42 8) (_ bv44 8))) :named a0))
+\<close>)
+  by (smt (cvc5))
+
+(*
+<s is translated into bvslt
+*)
+lemma "(42 :: 8 word) <s 44"
+  apply (test_smt_translate 
+\<open>
+(set-logic AUFBVLIRAFS)
+(assert (! (not (bvslt (_ bv42 8) (_ bv44 8))) :named a0))
+\<close>)
+  by (smt (cvc5))
+
+(*
+bit w n is translated into (= ((_ extract n n) w) #b1)
+*)
+lemma "bit (1705 :: 16 word) 3"
+  apply (test_smt_translate 
+\<open>
+(set-logic AUFBVLIRAFS)
+(assert (! (not (= ((_ extract 3 3) (_ bv1705 16)) (_ bv1 1))) :named a0))
+(assert (! (<= 0 3) :named a1))
+\<close>) supply[[smt_trace]]
+  by (smt (cvc5))
+
+
+
+context
+  includes bit_operations_syntax
+begin
+
+(*
+NOT is translated into bvnot
+*)
+lemma "(NOT (- 42 :: 32 word)) = 41"
+  apply (test_smt_translate 
+\<open>
+(set-logic AUFBVLIRAFS)
+(assert (! (not (= (bvnot (bvneg (_ bv42 32))) (_ bv41 32))) :named a0))
+\<close>)
+  by (smt (cvc5))
+
+(*
+AND is translated into bvand
+*)
+lemma "((41::32 word) AND (42 :: 32 word)) = 40"
+  apply (test_smt_translate 
+\<open>
+(set-logic AUFBVLIRAFS)
+(assert (! (not (= (bvand (_ bv41 32) (_ bv42 32)) (_ bv40 32))) :named a0))
+\<close>)
+  by (smt (cvc5))
+
+(*
+OR is translated into bvor
+*)
+lemma "((41::32 word) OR (42 :: 32 word)) = 43"
+  apply (test_smt_translate 
+\<open>
+(set-logic AUFBVLIRAFS)
+(assert (! (not (= (bvor (_ bv41 32) (_ bv42 32)) (_ bv43 32))) :named a0))
+\<close>)
+  by (smt (cvc5))
+
+(*
+XOR is translated into bvor
+*)
+lemma "((41::32 word) XOR (42 :: 32 word)) = 3"
+  apply (test_smt_translate 
+\<open>
+(set-logic AUFBVLIRAFS)
+(assert (! (not (= (bvxor (_ bv41 32) (_ bv42 32)) (_ bv3 32))) :named a0))
+\<close>)
+  by (smt (cvc5))
+
+(*
+push_bit is translated into bvshl
+For a nat constant, the constant is transformed into a word
+For a word variable with a nat cast the cast is removed  \<Longrightarrow> TODO
+Otherwise, we add a cast
+*)
+lemma "push_bit 3 (1705 :: 32 word) = 13640"
+  apply (test_smt_translate 
+\<open>
+(set-logic AUFBVLIRAFS)
+(assert (! (not (= (bvshl (_ bv1705 32) (_ bv3 32)) (_ bv13640 32))) :named a0))
+(assert (! (<= 0 3) :named a1))
+\<close>)
+  by (smt (cvc5))
+
+lemma "push_bit x (0 :: 32 word) = 0"
+  apply (test_smt_translate 
+\<open>
+(set-logic AUFBVLIRAFS)
+(declare-fun lift_x$ () Int)
+(assert (! (and (<= 0 lift_x$) (not (= (bvshl (_ bv0 32) ((_ int_to_bv 32) lift_x$)) (_ bv0 32)))) :named a0))
+(assert (! (and (<= 0 lift_x$) (<= 0 lift_x$)) :named a1))
+\<close>)
+  by (smt (cvc5))
+
+
+(*
+drop_bit is translated into bvshr
+For a nat constant, the constant is transformed into a word
+For a word variable with a nat cast the cast is removed  \<Longrightarrow> TODO
+Otherwise, we add a cast
+*)
+lemma "drop_bit 3 (1705 :: 16 word) = 213"
+  apply (test_smt_translate 
+\<open>
+(set-logic AUFBVLIRAFS)
+(assert (! (not (= (bvlshr (_ bv1705 16) (_ bv3 16)) (_ bv213 16))) :named a0))
+(assert (! (<= 0 3) :named a1))
+\<close>)
+  by (smt (cvc5))
+
+lemma "drop_bit x (0 :: 16 word) = 0"
+  apply (test_smt_translate 
+\<open>
+(set-logic AUFBVLIRAFS)
+(declare-fun lift_x$ () Int)
+(assert (! (and (<= 0 lift_x$) (not (= (bvlshr (_ bv0 16) ((_ int_to_bv 16) lift_x$)) (_ bv0 16)))) :named a0))
+(assert (! (and (<= 0 lift_x$) (<= 0 lift_x$)) :named a1))
+\<close>)
+  by (smt (cvc5))
+
+
+
+end
+
+
+
+
+
+
+
+
+
+
 
 
 lemma "Word.Word 0 = (0::5 word)"
